#number_theory
- $\sum_1^n(K^3) = (\sum_1^n(K))^2$

- $(2ab + 2bc + 2ca) = (a + b + c)^2 - (a^2 + b^2 + c^2)$
   **Example:**
   for $n$ numbers:
		$(a - b)^2 + (a - c)^2 + (b - c)^2 + ...$
		$= (n - 1)(a^2 + b^2 + c^2 + ...) - (2ab + 2bc + 2ca + ...)$
		$= (n)(a^2 + b^2 + c^2 + ...) - (a + b + c + ...)^2$



- 
$$
\begin{gathered}
\sum_{i=0}^{n}{\sum_{j=i+1}^{n}{(a_i*a_j)}} \\
	= \sum_{i=0}^{n}{(a_i * \sum_{j=i+1}^{n}{a_j})} \\
	= {(\sum_{i=0}^{n}{a_i})}^2 - \sum_{j=0}^{n}{(a_j^2)}
\end{gathered}
$$ 
   - **For more clarification**, revise the previous point in this file.
